This theorem could be proved by mathematical induction.
    \begin{proof}
        Start with the base case of $m = n = 1$, there are only 1 possible combination of event 1 and event 2.
        We move on to the case when $m = n = 2$, there are $4 = 2\times 2$ outcomes: $(1, 1), (1, 2), (2, 1), (2, 2)$.
        Suppose that the number of outcomes for each event are any integer $n \in \mathbb{N}^+$, similarly, we can enumerate all the cases from $(1, 1)$ to $(n, n)$,  $n^2 = n\times n$ outcomes.
        For the case when the number of outcomes coming to $n+1$. We can still enumerate all $(n+1)^2 = (n+1)\times(n+1)$ outcomes in a similar way.
        \par Therefore, the theorem is proven. This could be visualized by $$\begin{array}{l}(1,1),(1,2), \ldots,(1, n) \\(2,1),(2,2), \ldots,(2, n) \\\vdots \\(m, 1),(m, 2), \ldots,(m, n)\end{array}$$
    \end{proof}
